proofs/RandomLoop.fst
@@ -52,75 +52,74 @@ let variant (n : nat) : cond =
   fun (st, _, m) -> n <= 1000000 /\ st "n" == Nat 1000000 /\ st "i" == Nat n /\ st "j" == Nat n /\ m == Ok
 
 let pre_assign (k : nat) : cond = 
-  fun s -> variant k s /\ eval_expr s (Lt (Var "i") (Var "n")) == 0
+  fun s -> variant k s /\ eval_expr s (Lt (Var "i") (Var "n")) == 0 /\ s._3 == Ok
 
 let pre_assert : cond = 
   fun s -> exists (k : nat). variant k s
 
 // Lemas auxiliares
-let lemma_p_i_consequence (k:nat) (s:state)
-  : Lemma (requires mid_i k s)
-          (ensures (let st, hp, m = s in
-                   exists st_init. pre_assign k (st_init, hp, m) /\
-                   st "i" == Nat (eval_expr (st_init, hp, m) (Plus (Var "i") (Const 1))) /\
-                   (forall y. y <> "i" ==> st y == st_init y) /\
-                   m == Ok)) =
+let lemma_p_i_consequence (k : nat) (s : state) : Lemma 
+  (requires mid_i k s)
+  (ensures (is_ok (fun s ->
+      exists (st_init : var -> value). 
+        pre_assign k (st_init, s._2, s._3) /\ 
+        s._1 "i" == Nat (eval_expr (st_init, s._2, s._3) (Plus (Var "i") (Const 1))) /\
+        (forall y. y <> "i" ==> s._1 y == st_init y)) s)) =
   let st, hp, m = s in
   let st_init = override st "i" (Nat k) in
   let s_init = (st_init, hp, m) in
-  assert (eval_expr s_init (Var "i") == k)
+  let p_exist (st_i : var -> value) : prop =
+    pre_assign k (st_i, hp, m) /\ 
+    st "i" == Nat (eval_expr (st_i, hp, m) (Plus (Var "i") (Const 1))) /\
+    (forall y. y <> "i" ==> st y == st_i y)
+  in
+  Classical.exists_intro p_exist st_init
 
-let lemma_p_j_consequence (k:nat) (s:state)
-  : Lemma (requires variant (k + 1) s)
-          (ensures (let st, hp, m = s in
-                   exists st_init. mid_i k (st_init, hp, m) /\
-                   st "j" == Nat (eval_expr (st_init, hp, m) (Plus (Var "j") (Const 1))) /\
-                   (forall y. y <> "j" ==> st y == st_init y) /\
-                   m == Ok)) =
+let lemma_p_j_consequence (k:nat) (s:state) : Lemma 
+  (requires variant (k + 1) s)
+  (ensures (is_ok (fun s ->
+      exists (st_init : var -> value). 
+        mid_i k (st_init, s._2, s._3) /\ 
+        s._1 "j" == Nat (eval_expr (st_init, s._2, s._3) (Plus (Var "j") (Const 1))) /\
+        (forall y. y <> "j" ==> s._1 y == st_init y)) s)) =
   let st, hp, m = s in
   let st_init = override st "j" (Nat k) in
   let s_init = (st_init, hp, m) in
-  assert (eval_expr s_init (Var "j") == k)
+  let p_exist (st_i : var -> value) : prop =
+    mid_i k (st_i, hp, m) /\ 
+    st "j" == Nat (eval_expr (st_i, hp, m) (Plus (Var "j") (Const 1))) /\
+    (forall y. y <> "j" ==> st y == st_i y)
+  in
+  Classical.exists_intro p_exist st_init
 
-let proof_loop_step (k : nat) : isl_triple (variant k) loop_body (variant (k + 1)) =
+let proof_loop_step (k : nat) : isl_triple (is_ok (variant k)) loop_body (variant (k + 1)) =
   let p_assumed = ISL_Assume #(variant k) (Lt (Var "i") (Var "n")) in
 
   let p_i_raw = ISL_Assign #(pre_assign k) "i" (Plus (Var "i") (Const 1)) in
-  let _ = forall_intro (move_requires (lemma_p_i_consequence k)) in
-  let p_i = ISL_Consequence (pre_assign k) (mid_i k) p_i_raw () () in
+  let pf_i = Classical.forall_intro (Classical.move_requires (lemma_p_i_consequence k)) in
+  let p_i = ISL_Consequence (pre_assign k) (mid_i k) p_i_raw () pf_i in
 
   let p_j_raw = ISL_Assign #(mid_i k) "j" (Plus (Var "j") (Const 1)) in
-  let _ = forall_intro (move_requires (lemma_p_j_consequence k)) in
-  let p_j_branch = ISL_Consequence (mid_i k) (variant (k + 1)) p_j_raw () () in
+  let pf_j = Classical.forall_intro (Classical.move_requires (lemma_p_j_consequence k)) in
+  let p_j_branch = ISL_Consequence (mid_i k) (variant (k + 1)) p_j_raw () pf_j in
+  
   let p_j = ISL_ChoiceL p_j_branch in
-  let p_j' = 
-    ISL_Consequence (fun s -> s._3 == Ok /\ mid_i k s) (variant (k + 1)) p_j () ()
-  in
-  let p_ij = ISL_Seq p_i p_j' in
+  let p_ij = ISL_Seq p_i p_j in
 
-  let expected_pre_ij (s:state) : prop = 
-    s._3 == Ok /\ (s._3 == Ok /\ variant k s /\ eval_expr s (Lt (Var "i") (Var "n")) == 0)
-  in
-  let expected_post_ij (s:state) : prop =
-    variant (k + 1) s \/ s._3 == Er /\ mid_i k s
-  in
+  let mid_assumed : cond = fun s -> variant k s /\ eval_expr s (Lt (Var "i") (Var "n")) == 0 in
+  let expected_post_ij : cond = fun s -> variant (k + 1) s \/ s._3 == Er /\ mid_i k s in
 
-  let p_ij_adapted = ISL_Consequence 
-    expected_pre_ij 
-    expected_post_ij 
-    p_ij 
-    () () 
+  let p_ij_adapted = 
+    ISL_Consequence #(pre_assign k) (is_ok mid_assumed) expected_post_ij p_ij () () 
   in
+  
   let p_raw = ISL_Seq p_assumed p_ij_adapted in
   ISL_Consequence (variant k) (variant (k + 1)) p_raw () ()
 
-let lemma_kleene : isl_triple 
-  (fun s -> variant 0 s /\ s._3 == Ok) 
-  (Kleene loop_body) 
-  (fun s -> exists (k:nat). variant k s /\ (k == 0 ==> s._3 == Ok)) =
+let lemma_kleene : isl_triple (kleene_pre variant) (Kleene loop_body) (kleene_post variant) =
   let step (n : nat) =
     ISL_Consequence
-      (fun s -> variant n s /\ s._3 == Ok)
+      (variant n)
       (variant (n + 1))
       (proof_loop_step n)
       () ()
@@ -131,39 +130,37 @@ let mid_n (s : state) : prop =
   s._3 == Ok /\ s._1 "n" == Nat 1000000
 
 // Demostraciones formales
-let proof_init : isl_triple pre_vacia init_vars (variant 0) =
+let proof_init : isl_triple (is_ok pre_vacia) init_vars (kleene_pre variant) =
   let p_n_raw = ISL_Assign #pre_vacia "n" (Const 1000000) in
   let p_n = ISL_Consequence pre_vacia mid_n p_n_raw () () in
-  
+
   let p_i = ISL_Assign #_ "i" (Const 0) in
   let p_j = ISL_Assign #_ "j" (Const 0) in
-
+  
   let p_ij = ISL_Seq p_i p_j in
   let p_init = ISL_Seq p_n p_ij in
+  ISL_Consequence pre_vacia (kleene_pre variant) p_init () ()
 
-  ISL_Consequence pre_vacia (variant 0) p_init () ()
-
-let proof_assert : isl_triple pre_assert (Seq (Assume (Eq (Var "i") (Var "n"))) assert_stmt) post_er_bug =
+let proof_assert : isl_triple (is_ok pre_assert) (Seq (Assume (Eq (Var "i") (Var "n"))) assert_stmt) post_er_bug =
   let p_exit_raw = ISL_Assume #pre_assert (Eq (Var "i") (Var "n")) in
   let p_exit = ISL_Consequence pre_assert (variant 1000000) p_exit_raw () () in
-
-  let p_cond_err = ISL_Assume #(fun s -> s._3 == Ok /\ variant 1000000 s) (Eq (Var "j") (Var "n")) in
-  let p_err = ISL_Error #_ in
-  let p_branch_err = ISL_Seq p_cond_err p_err in
-
+  
+  let p_cond_err_raw = ISL_Assume #(variant 1000000) (Eq (Var "j") (Var "n")) in
+  let pre_error_state : cond = fun s -> variant 1000000 s /\ eval_expr s (Eq (Var "j") (Var "n")) == 0 in
+  let p_cond_err = ISL_Consequence (variant 1000000) pre_error_state p_cond_err_raw () () in
+  let p_err_raw = ISL_Error #pre_error_state in
+  
+  let p_branch_err_raw = ISL_Seq p_cond_err p_err_raw in
+  let p_branch_err = ISL_Consequence (variant 1000000) post_er_bug p_branch_err_raw () () in
+  
   let p_assert = ISL_ChoiceL p_branch_err in
   let p_raw = ISL_Seq p_exit p_assert in
   ISL_Consequence pre_assert post_er_bug p_raw () ()
 
-let proof_prog1 : isl_triple pre_vacia prog1 post_er_bug =
-  let expected_pre_assert (s:state) : prop =
-    s._3 == Ok /\ (exists (k: nat). variant k s /\ (k == 0 ==> s._3 == Ok))
-  in
-  let adapted_assert = ISL_Consequence expected_pre_assert post_er_bug proof_assert () () in
-  let p_kleene_assert = ISL_Seq lemma_kleene adapted_assert in
-  let expected_pre_kleene (s:state) : prop =
-    s._3 == Ok /\ variant 0 s
-  in
-  let adapted_kleene_assert = ISL_Consequence expected_pre_kleene post_er_bug p_kleene_assert () () in
-  let triple_seq = proof_init `ISL_Seq` adapted_kleene_assert in
-  ISL_Consequence pre_vacia post_er_bug triple_seq () ()
+let proof_prog1 : isl_triple (is_ok pre_vacia) prog1 post_er_bug =
+  let adapted_assert = ISL_Consequence (kleene_post variant) post_er_bug proof_assert () () in
+  let p_kleene_assert_raw = ISL_Seq lemma_kleene adapted_assert in
+  let p_kleene_assert = ISL_Consequence (kleene_pre variant) post_er_bug p_kleene_assert_raw () () in
+  
+  let p_raw = ISL_Seq proof_init p_kleene_assert in
+  ISL_Consequence pre_vacia post_er_bug p_raw () ()
