proofs/AllocFree.fst
@@ -17,34 +17,30 @@ let post_alloc (s : state) : prop =
     points_to l v s /\
     (exists x_old. emp (override s._1 "x" x_old, override s._2 l Empty, Ok))
 
-let pre_free (s:state) : prop = 
-  s._3 == Ok /\ post_alloc s
-
 let post_free (s : state) : prop =
   exists (v : value). 
     s._3 == Ok /\
     points_to_empty (eval_expr s (Var "x")) s /\
-    pre_free (s._1, override s._2 (eval_expr s (Var "x")) (Full v), Ok)
-
-let pre_store (s : state) : prop =
-  s._3 == Ok /\ post_free s
+    post_alloc (s._1, override s._2 (eval_expr s (Var "x")) (Full v), Ok)
 
 let post_uaf_err (s : state) : prop =
   s._3 == Er /\ 
   points_to_empty (eval_expr s (Var "x")) s /\
-  pre_store (s._1, s._2, Ok)
+  post_free (s._1, s._2, Ok)
 
 let prog_uaf =
   (Alloc "x") `Seq`
   ((Free (Var "x")) `Seq`
   (Store (Var "x") (Const 1)))
 
-let proof_uaf : isl_triple emp prog_uaf post_uaf_err =
-  let p_alloc = ISL_Alloc1 #emp "x" in
-  let p_free_raw = ISL_Free #pre_free (Var "x") in
-  let p_store = ISL_StoreEr #pre_store (Var "x") (Const 1) in
+let proof_uaf : isl_triple (is_ok emp) prog_uaf post_uaf_err =
+  let p_alloc_raw = ISL_Alloc1 #emp "x" in
+  let p_alloc = ISL_Consequence emp post_alloc p_alloc_raw () () in
 
-  let p_free = ISL_Consequence pre_free post_free p_free_raw () () in
+  let p_free_raw = ISL_Free #post_alloc (Var "x") in
+  let p_store = ISL_StoreEr #post_free (Var "x") (Const 1) in
+
+  let p_free = ISL_Consequence post_alloc post_free p_free_raw () () in
 
   let p_seq1 = ISL_Seq p_free p_store in
   let p_seq2 = ISL_Seq p_alloc p_seq1 in
