proofs/ListSumLen.fst
@@ -41,8 +41,8 @@ let n_target = 10
 
 let pre_vacia (start_ptr : loc) : cond = 
   fun s -> let xs = ones n_target in
-    s._3 == Ok /\ 
     (exists (curr_ptr : loc). 
+      s._3 == Ok /\
       s._1 "ptr" == Loc curr_ptr /\ 
       (let l_visit, l_remain = splitAt 0 xs in
       (list_seq start_ptr curr_ptr l_visit ** list_seq curr_ptr 0 l_remain)) s)
@@ -60,7 +60,7 @@ let variant (start_ptr : loc) (k : nat) : cond =
 let mid_sum (start_ptr : loc) : cond = 
   fun s -> pre_vacia start_ptr s /\ s._1 "sum" == Nat 0
 
-let proof_init (start_ptr: loc) : isl_triple (pre_vacia start_ptr) init_vars (kleene_pre (variant start_ptr)) =
+let proof_init (start_ptr: loc) : isl_triple (is_ok (pre_vacia start_ptr)) init_vars (kleene_pre (variant start_ptr)) =
   let pre = pre_vacia start_ptr in
   let mid = mid_sum start_ptr in 
   let post = kleene_pre (variant start_ptr) in
@@ -68,204 +68,8 @@ let proof_init (start_ptr: loc) : isl_triple (pre_vacia start_ptr) init_vars (kl
   let p_sum_raw = ISL_Assign #pre "sum" (Const 0) in
   let p_sum = ISL_Consequence pre mid p_sum_raw () () in
   
-  let p_len_raw = ISL_Assign #(fun s -> s._3 == Ok /\ mid s) "len" (Const 0) in
-  let p_len : isl_triple (fun s -> s._3 == Ok /\ mid s) (Assign "len" (Const 0)) post = 
-    ISL_Consequence (fun s -> s._3 == Ok /\ mid s) post p_len_raw () () 
-  in
+  let p_len_raw = ISL_Assign #mid "len" (Const 0) in
+  let p_len = ISL_Consequence mid post p_len_raw () () in
   
   let p_seq = ISL_Seq p_sum p_len in
   ISL_Consequence pre post p_seq () ()
-
-let lemma_sep_indep (p q : cond) (st1 st2 : store) (hp : heap) (m1 m2 : term_mode)
-  : Lemma (requires (forall h. p (st1, h, m1) <==> p (st2, h, m2)) /\
-                    (forall h. q (st1, h, m1) <==> q (st2, h, m2)))
-          (ensures (p ** q) (st1, hp, m1) <==> (p ** q) (st2, hp, m2)) = ()
-
-let rec lemma_list_seq_indep (i j : loc) (xs : list value) (st1 st2 : store) (hp : heap) (m1 m2 : term_mode)
-  : Lemma (ensures list_seq i j xs (st1, hp, m1) <==> list_seq i j xs (st2, hp, m2))
-          (decreases xs) =
-  match xs with
-  | [] -> ()
-  | x :: xss ->
-    let prove_rec (next_j : loc) (h : heap)
-      : Lemma (list_seq next_j j xss (st1, h, m1) <==> list_seq next_j j xss (st2, h, m2)) =
-      lemma_list_seq_indep next_j j xss st1 st2 h m1 m2
-    in
-    let prove_rec_h (next_j : loc)
-      : Lemma (forall (h : heap). list_seq next_j j xss (st1, h, m1) <==> list_seq next_j j xss (st2, h, m2)) =
-      Classical.forall_intro (prove_rec next_j)
-    in
-    Classical.forall_intro prove_rec_h;
-    
-    let p_A = points_to i x in
-    let p_B (next_j : loc) = points_to (i + 1) (Loc next_j) in
-    let p_C (next_j : loc) = list_seq next_j j xss in
-    let p_AB (next_j : loc) : cond = p_A ** p_B next_j in
-    let p_body (next_j : loc) : cond = fun s -> (p_AB next_j ** p_C next_j) s in
-
-    let prove_body (next_j : loc)
-      : Lemma (p_body next_j (st1, hp, m1) <==> p_body next_j (st2, hp, m2)) =
-      let prove_C (h : heap) : Lemma (p_C next_j (st1, h, m1) <==> p_C next_j (st2, h, m2)) =
-        lemma_list_seq_indep next_j j xss st1 st2 h m1 m2
-      in
-      Classical.forall_intro prove_C;
-
-      let prove_AB (h : heap) : Lemma (p_AB next_j (st1, h, m1) <==> p_AB next_j (st2, h, m2)) =
-        lemma_sep_indep p_A (p_B next_j) st1 st2 h m1 m2
-      in
-      Classical.forall_intro prove_AB;
-      lemma_sep_indep (p_AB next_j) (p_C next_j) st1 st2 hp m1 m2
-    in
-
-    Classical.forall_intro prove_body
-
-let p_fr_mem (start_ptr : loc) (k : nat) (curr_ptr : loc) (next_j : loc) : cond =
-  fun s ->
-    let xs = ones n_target in
-    let l_visit, l_remain = splitAt k xs in
-    match l_remain with
-    | [] -> False
-    | _ :: tl ->
-      (points_to (curr_ptr + 1) (Loc next_j) ** 
-       list_seq start_ptr curr_ptr l_visit ** 
-       list_seq next_j 0 tl) s
-
-let fr_load (start_ptr : loc) (k : nat) : cond =
-  fun s ->
-    k < n_target /\ s._1 "sum" == Nat k /\ s._1 "len" == Nat k /\
-    (exists (curr_ptr next_j: loc).
-      s._1 "ptr" == Loc curr_ptr /\
-      p_fr_mem start_ptr k curr_ptr next_j s)
-
-let lemma_fr_mem_indep (start_ptr : loc) (k : nat) (curr_ptr : loc) (next_j : loc) (st1 st2 : store) (hp : heap) (m1 m2 : term_mode)
-  : Lemma (p_fr_mem start_ptr k curr_ptr next_j (st1, hp, m1) <==> p_fr_mem start_ptr k curr_ptr next_j (st2, hp, m2)) =
-  let xs = ones n_target in
-  let l_visit, l_remain = splitAt k xs in
-  match l_remain with
-  | [] -> ()
-  | _ :: tl ->
-    let p_A = points_to (curr_ptr + 1) (Loc next_j) in
-    let p_B = list_seq start_ptr curr_ptr l_visit in
-    let p_C = list_seq next_j 0 tl in
-    let p_AB : cond = p_A ** p_B in
-
-    let prove_A (h : heap) : Lemma (p_A (st1, h, m1) <==> p_A (st2, h, m2)) = () in
-    Classical.forall_intro prove_A;
-
-    let prove_B (h : heap) : Lemma (p_B (st1, h, m1) <==> p_B (st2, h, m2)) =
-      lemma_list_seq_indep start_ptr curr_ptr l_visit st1 st2 h m1 m2
-    in
-    Classical.forall_intro prove_B;
-
-    let prove_C (h : heap) : Lemma (p_C (st1, h, m1) <==> p_C (st2, h, m2)) =
-      lemma_list_seq_indep next_j 0 tl st1 st2 h m1 m2
-    in
-    Classical.forall_intro prove_C;
-
-    let prove_AB (h : heap) : Lemma (p_AB (st1, h, m1) <==> p_AB (st2, h, m2)) =
-      lemma_sep_indep p_A p_B st1 st2 h m1 m2
-    in
-    Classical.forall_intro prove_AB;
-    lemma_sep_indep p_AB p_C st1 st2 hp m1 m2
-
-let pf_indep_load (start_ptr : loc) (k : nat)
-  : squash (independent_on_vars (modifies (Load "v" (Var "ptr"))) (fr_load start_ptr k)) =
-
-  let prove_indep (st1 st2 : store) (hp : heap) (m1 m2 : term_mode)
-    : Lemma (requires match_except_vars (modifies (Load "v" (Var "ptr"))) st1 st2)
-            (ensures fr_load start_ptr k (st1, hp, m1) <==> fr_load start_ptr k (st2, hp, m2)) =
-
-    let prove_mem (curr_ptr : loc) (next_j : loc)
-      : Lemma (p_fr_mem start_ptr k curr_ptr next_j (st1, hp, m1) <==> p_fr_mem start_ptr k curr_ptr next_j (st2, hp, m2)) =
-      lemma_fr_mem_indep start_ptr k curr_ptr next_j st1 st2 hp m1 m2
-    in
-
-    Classical.forall_intro (fun c -> Classical.forall_intro (prove_mem c))
-  in
-
-  let prove_indep_impl (st1 st2 : store) (hp : heap) (m1 m2 : term_mode)
-    : Lemma (match_except_vars (modifies (Load "v" (Var "ptr"))) st1 st2 ==>
-            (fr_load start_ptr k (st1, hp, m1) <==> fr_load start_ptr k (st2, hp, m2))) =
-    Classical.move_requires (prove_indep st1 st2 hp m1) m2
-  in
-  
-  Classical.forall_intro (fun st1 ->
-    Classical.forall_intro (fun st2 ->
-      Classical.forall_intro (fun hp ->
-        Classical.forall_intro (fun m1 ->
-          Classical.forall_intro (fun m2 -> prove_indep_impl st1 st2 hp m1 m2)))))
-
-let pre_loop (start_ptr : loc) (k : nat) (s : state) : prop =
-  variant start_ptr k s /\ s._3 == Ok
-
-let mid_assume (start_ptr : loc) (k : nat) (s : state) : prop =
-  s._3 == Ok /\ pre_loop start_ptr k s /\
-  eval_expr s (enot (Eq (Var "ptr") (Const 0))) == 0
-
-let mid_load_v (start_ptr : loc) (k : nat) : cond =
-  fun s -> let xs = ones n_target in
-    k < n_target /\ s._3 == Ok /\
-    s._1 "v" == Nat 1 /\
-    s._1 "sum" == Nat k /\ s._1 "len" == Nat k /\
-    (exists (curr_ptr next_j : loc).
-      s._1 "ptr" == Loc curr_ptr /\
-      (let l_visit, l_remain = splitAt k xs in
-      match l_remain with
-      | [] -> (fun _ -> False)
-      | _ :: tl ->
-        (points_to curr_ptr (Nat 1) ** points_to (curr_ptr + 1) (Loc next_j) **
-        list_seq start_ptr curr_ptr l_visit ** list_seq next_j 0 tl)) s)
-
-let mid_load_v_ext (start_ptr : loc) (k : nat) (s : state) : prop =
-  mid_load_v start_ptr k s /\ eval_expr s (enot (Eq (Var "ptr") (Const 0))) == 0
-
-let proof_step1_assume (start_ptr : loc) (k : nat)
-  : isl_triple (pre_loop start_ptr k) 
-               (Assume (enot (Eq (Var "ptr") (Const 0)))) 
-               (mid_assume start_ptr k) =
-  ISL_Assume #(pre_loop start_ptr k) (enot (Eq (Var "ptr") (Const 0)))
-
-let proof_step2_load_v (start_ptr : loc) (k : nat)
-  : isl_triple (mid_assume start_ptr k) 
-               (Load "v" (Var "ptr")) 
-               (mid_load_v_ext start_ptr k) =
-
-  let stmt_load = Load "v" (Var "ptr") in
-
-  let pre_load_v (s : state) : prop = 
-    s._3 == Ok /\ (exists (p : loc). s._1 "ptr" == Loc p /\ points_to p (Nat 1) s) /\
-    eval_expr s (enot (Eq (Var "ptr") (Const 0))) == 0
-  in
-    
-  let p_load_base = ISL_Load #pre_load_v "v" (Var "ptr") in
-
-  let post_load_base (s : state) : prop =
-    exists l v x_old. s._3 == Ok /\ eval_expr (override s._1 "v" x_old, s._2, Ok) (Var "ptr") == l /\
-      points_to l v s /\ s._1 "v" == v /\ pre_load_v (override s._1 "v" x_old, s._2, Ok)
-  in
-  
-  let p_load_framed = ISL_Frame #pre_load_v #stmt_load #post_load_base (fr_load start_ptr k) p_load_base (pf_indep_load start_ptr k) in
-  
-  let pf_load_pre (s : state)
-    : Lemma (requires (pre_load_v ** fr_load start_ptr k) s) 
-            (ensures mid_assume start_ptr k s) = 
-    admit()
-  in
-  
-  let pf_load_post (s : state)
-    : Lemma (requires mid_load_v_ext start_ptr k s) 
-            (ensures (post_load_base ** fr_load start_ptr k) s) = 
-    admit()
-  in
-  
-  let sq_pre_load () : squash (forall x. (pre_load_v ** fr_load start_ptr k) x ==> mid_assume start_ptr k x) =
-    Classical.forall_intro (Classical.move_requires pf_load_pre)
-  in
-  
-  let sq_post_load () : squash (forall x. mid_load_v_ext start_ptr k x ==> (post_load_base ** fr_load start_ptr k) x) =
-    Classical.forall_intro (Classical.move_requires pf_load_post)
-  in
-  
-  ISL_Consequence #(pre_load_v ** fr_load start_ptr k) #stmt_load #(post_load_base ** fr_load start_ptr k) 
-                  (mid_assume start_ptr k) (mid_load_v_ext start_ptr k) 
-                  p_load_framed (sq_pre_load ()) (sq_post_load ())
