proofs/PushBack.fst
@@ -16,7 +16,7 @@ let client (ptr : var) : stmt =
 
 let pre_client (ptr : var) (s : state) : prop =
   exists (l_v : loc) (l_a : loc) (val_a : value).
-    s._3 == Ok /\ s._1 ptr == Loc l_v /\
+    s._1 ptr == Loc l_v /\
     (points_to l_v (Loc l_a) ** points_to l_a val_a) s
 
 let post_load_x (ptr : var) (s : state) : prop =
@@ -59,14 +59,13 @@ let post_err (ptr : var) (s : state) : prop =
   points_to_empty (eval_expr s (Var "x")) s /\
   post_store_v ptr (s._1, s._2, Ok)
 
-let proof_client (ptr : var) : isl_triple (pre_client ptr) (client ptr) (post_err ptr) =
+let proof_client (ptr : var) : isl_triple (is_ok (pre_client ptr)) (client ptr) (post_err ptr) =
   
   let p_load_x_raw = ISL_Load #(pre_client ptr) "x" (Var ptr) in
   let p_load_x = ISL_Consequence (pre_client ptr) (post_load_x ptr) p_load_x_raw () () in
 
-  let pre_y = fun (s : state) -> s._3 == Ok /\ post_load_x ptr s in
-  let p_load_y_raw = ISL_Load #pre_y "y" (Var ptr) in
-  let p_load_y = ISL_Consequence pre_y (post_load_y ptr) p_load_y_raw () () in
+  let p_load_y_raw = ISL_Load #(post_load_x ptr) "y" (Var ptr) in
+  let p_load_y = ISL_Consequence (post_load_x ptr) (post_load_y ptr) p_load_y_raw () () in
 
   let p_free_y = ISL_Free (Var "y") in
   let p_alloc_y = ISL_Alloc1 "y" in
@@ -77,15 +76,14 @@ let proof_client (ptr : var) : isl_triple (pre_client ptr) (client ptr) (post_er
   let p_seq_pb1 = ISL_Seq p_load_y p_seq_pb2 in
 
   let p_push_back_raw = ISL_ChoiceL p_seq_pb1 in
-  let p_push_back = ISL_Consequence pre_y (post_store_v ptr) p_push_back_raw () () in
+  let p_push_back = ISL_Consequence (post_load_x ptr) (post_store_v ptr) p_push_back_raw () () in
 
-  let pre_err_step = fun (s : state) -> s._3 == Ok /\ post_store_v ptr s in
-  let p_store_err_raw = ISL_StoreEr #pre_err_step (Var "x") (Const 88) in
-  let p_store_err = ISL_Consequence pre_err_step (post_err ptr) p_store_err_raw () () in
+  let p_store_err_raw = ISL_StoreEr #(post_store_v ptr) (Var "x") (Const 88) in
+  let p_store_err = ISL_Consequence (post_store_v ptr) (post_err ptr) p_store_err_raw () () in
 
   let p_client_seq2 = ISL_Seq p_push_back p_store_err in
   
-  let p_client_raw : isl_triple (pre_client ptr) (client ptr) 
+  let p_client_raw : isl_triple (is_ok (pre_client ptr)) (client ptr) 
     (fun s -> post_err ptr s \/ (s._3 == Er /\ post_store_v ptr s) \/ (s._3 == Er /\ post_load_x ptr s)) = 
     ISL_Seq p_load_x p_client_seq2 
   in
